### 1.2.11.3 一些近似计算

- 记号

$$
\begin{aligned}
    P(n) & = 1 + \frac{n-1}{n} + \frac{n-2}{n} \frac{n-2}{n-1} + \cdots = \sum_{k=0}^n{\frac{(n-k)^k (n-k)!}{n!}} \\
    Q(n) & = 1 + \frac{n-1}{n} + \frac{n-1}{n} \frac{n-2}{n} + \cdots = \sum_{k=1}^n{\frac{n!}{(n-k)! n^k}} \\
    R(n) & = 1 + \frac{n}{n+1} + \frac{n}{n+1} \frac{n}{n+2} + \cdots = \sum_{k \ge 0}{\frac{n! n^k}{(n+k)!}}
\end{aligned}
$$

- 结果

$$
\begin{aligned}
&P(n)=\sqrt{\frac{\pi n}{2}}-\frac{2}{3}+\frac{11}{24} \sqrt{\frac{\pi}{2 n}}+\frac{4}{135 n}-\frac{71}{1152} \sqrt{\frac{\pi}{2 n^{3}}}+O\left(n^{-2}\right)\\
&Q(n)=\sqrt{\frac{\pi n}{2}}-\frac{1}{3}+\frac{1}{12} \sqrt{\frac{\pi}{2 n}}-\frac{4}{135 n}+\frac{1}{288} \sqrt{\frac{\pi}{2 n^{3}}}+O\left(n^{-2}\right)\\
&R(n)=\sqrt{\frac{\pi n}{2}}+\frac{1}{3}+\frac{1}{12} \sqrt{\frac{\pi}{2 n}}+\frac{4}{135 n}+\frac{1}{288} \sqrt{\frac{\pi}{2 n^{3}}}+O\left(n^{-2}\right)
\end{aligned}
$$

### 习题

> 1

$n = 0$时，$f(x) = f(0) + \int_0^x{f'(x-t)dt} = f(0) + \int_x^0{-f'(u)du} = f(0) + \int_0^x{f'(u)du} = f(0) + f(x) - f(0) = f(x)$。

n时
$$
f(x) = f(0) + f'(0)x + \cdots + \frac{f^{(n)}(0)x^n}{n!} + \int_0^x{\frac{t^n}{n!} f^{(n+1)}(x-t) dt}
$$
n+1时
$$
\begin{aligned}
	& f(0) + f'(0)x + \cdots + \frac{f^{(n)}(0)x^n}{n!} + \frac{f^{(n+1)}(0)x^{n+1}}{(n+1)!} + \int_0^x{\frac{t^{n+1}}{(n+1)!} f^{(n+2)}(x-t) dt} \\
	= & f(x) - \int_0^x{\frac{t^n}{n!} f^{(n+1)}(x-t) dt} + \frac{f^{(n+1)}(0)x^{n+1}}{(n+1)!} + \int_0^x{\frac{t^{n+1}}{(n+1)!} f^{(n+2)}(x-t) dt} \\
	= & f(x) - \int_0^x{\frac{(x-u)^n}{n!} f^{(n+1)}(u) dt} + \frac{f^{(n+1)}(0)x^{n+1}}{(n+1)!} + \int_0^x{\frac{(x-u)^{n+1}}{(n+1)!} f^{(n+2)}(u) dt} \\
	= & f(x) + \frac{f^{(n+1)}(0)x^{n+1}}{(n+1)!} + \frac{1}{(n+1)!} \left[(x-u)^{n+1} \cdot f^{(n+1)}(u) \right]^x_0 \\
	= & f(x) + \frac{f^{(n+1)}(0)x^{n+1}}{(n+1)!} - \frac{1}{(n+1)!}x^{n+1}f^{(n+1)}(0) \\
	= & f(x)
\end{aligned}
$$

> 2

$$
\begin{aligned}
	\gamma(a,x) 
	& = \int_0^x{e^{-t} t^{a-1} dt} \\
	& = \int_0^x{(1 - t + \frac{t^2}{2!} - \frac{t^3}{3!} + \cdots)t^{a-1}dt} \\
	& = \int_0^x{(t^{a-1} - t^a + \frac{t^{a+1}}{2!} - \frac{t^{a+2}}{3!} + \cdots)dt} \\
	& = \frac{1}{a} x^a - \frac{1}{a+1} x^{a+1} + \frac{2!(a+2)} x^{a+2} + \cdots
\end{aligned}
$$

